modifying the file structure of rbpf and adding 32 info as well as some proof

benchmark/clightlogicexample.c
@@ -1,0 +1,111 @@
+#include "clightlogicexample.h"
+
+static void upd_pc_incr(struct bpf_state* st) {
+  (*st).state_pc = (*st).state_pc+1;
+  return ;
+}
+
+static void upd_reg (struct bpf_state* st, unsigned int i, unsigned long long v){
+  (*st).regsmap[i] = v;
+  return ;
+}
+
+static void upd_flag(struct bpf_state* st, int f){
+  (*st).bpf_flag = f;
+  return ;
+}
+
+static struct memory_region *eval_mem_regions(struct bpf_state* st){
+  return (*st).mrs;
+}
+
+
+unsigned long long list_get(unsigned long long *l, int idx)
+{
+  return *(l + idx);
+}
+
+struct memory_region *get_mem_region(struct bpf_state* st, unsigned int n)
+{
+  struct memory_region *mrs;
+  mrs = eval_mem_regions(st);
+  return mrs + n;
+}
+
+int get_immediate(unsigned long long ins)
+{
+  return (int) (ins >> 32LLU);
+}
+
+unsigned char get_opcode_mem_ld_imm(unsigned char op)
+{
+  return (unsigned char) (op & 255);
+}
+
+unsigned int get_add(unsigned int x, unsigned int y)
+{
+  return x + y;
+}
+
+unsigned int get_addr_ofs(unsigned long long x, int ofs)
+{
+  return (unsigned int) (x + (unsigned long long) ofs);
+}
+
+_Bool is_well_chunk_bool(unsigned int chunk)
+{
+  switch (chunk) {
+    case 1:
+      return 1;
+    case 2:
+      return 1;
+    case 4:
+      return 1;
+    case 8:
+      return 1;
+    default:
+      return 0;
+    
+  }
+}
+
+unsigned int calc_sum(unsigned int v, unsigned int n)
+{
+  unsigned int n1;
+  unsigned int nv;
+  if (n == 0U) {
+    return 0U;
+  } else {
+    n1 = n - 1U;
+    nv = get_add(v, 1U);
+    return calc_sum(nv, n1);
+  }
+}
+
+void step_opcode_mem_ld_imm(struct bpf_state* st, int imm, int pc, int len, unsigned int dst, unsigned char op, unsigned long long *l)
+{
+  unsigned char opcode_ld;
+  unsigned long long next_ins;
+  int next_imm;
+  opcode_ld = get_opcode_mem_ld_imm(op);
+  switch (opcode_ld) {
+    case 24:
+      if (pc + 1 < len) {
+        next_ins = list_get(l, pc + 1);
+        next_imm = get_immediate(next_ins);
+        upd_reg(st, dst,
+                (unsigned long long) (unsigned int) imm
+                  | (unsigned long long) (unsigned int) next_imm << 32U);
+        upd_pc_incr(st);
+        upd_flag(st, 0);
+        return;
+      } else {
+        upd_flag(st, -5);
+        return;
+      }
+    default:
+      upd_flag(st, -1);
+      return;
+    
+  }
+}
