benchmark/clightlogicexample.h
@@ -1,0 +1,16 @@
+#include<stdio.h>
+
+struct memory_region {
+  unsigned int start_addr;
+  unsigned int block_size;
+  unsigned int block_perm;
+  unsigned int block_ptr;
+};
+
+struct bpf_state {
+  unsigned int state_pc;
+  int bpf_flag;
+  unsigned int mem_num;
+  unsigned long long regsmap[11];
+  struct memory_region *mrs;
+};
