benchmark/BenchmarkTests.v
@@ -1,0 +1,72 @@
+From Coq Require Import BinNums List Ascii String Nat ZArith.
+From Coq Require Import Numbers.AltBinNotations.
+Import List.ListNotations.
+
+From compcert.cfrontend Require Csyntax Ctypes.
+From compcert.common Require Import Errors Values.
+From compcert.lib Require Import Integers.
+ 
+
+From dx Require Import ResultMonad IR CoqIR IRtoC DXModule DumpAsC.
+From dx.Type Require Bool Nat.
+From bpf.src Require Import DxIntegers DxList64 DxValues DxRegs DxState DxOpcode DxMonad DxFlag DxAST DxMemRegion DxMemType DxInstructions.
+
+Open Scope monad_scope.
+Fixpoint calc_sum (v: valu32_t) (n:nat){struct n}: M valu32_t :=
+  match n with
+  | O => returnM val32_zero
+  | S n1 =>
+    do nv <- get_add v val32_one;
+      calc_sum nv n1
+  end.
+
+Close Scope monad_scope.
+
+(***************************************)
+
+
+GenerateIntermediateRepresentation SymbolIRs
+  M bindM returnM
+  Bool.Exports
+  Nat.Exports
+  DxIntegers.Exports
+  DxList64.Exports
+  DxValues.Exports
+  DxRegs.Exports
+  DxState.Exports
+  DxOpcode.Exports
+  DxFlag.Exports
+  DxAST.Exports
+  DxMemRegion.Exports
+  DxMemType.Exports
+  upd_pc_incr
+  upd_reg
+  upd_flag
+  eval_mem_regions
+  __
+  (**r to test if `Coq list` to `C array` is ok? *)
+  list_get
+  (**r read memory_region *)
+  get_mem_region
+  (**r 1. check complex expression in the return statement *)
+  get_immediate
+  (**r *)
+  get_opcode_mem_ld_imm
+  (**r the simplest function: a + b *)
+  get_add
+  (**r 2. check complex expression in the return statement *)
+  get_addr_ofs
+  (**r check switch-case *)
+  is_well_chunk_bool
+  (**r complex function: including `get_add` and recursion *)
+  calc_sum
+  step_opcode_mem_ld_imm
+.
+(*
+Definition dxModuleTest := makeDXModuleWithDefaults SymbolIRs.*)
+
+Definition dxModuleTest := makeDXModuleWithUserIds 
+  [ mem_region_def; state_struct_def]
+  [
+   "memory_region"; "start_addr"; "block_size"; "block_perm"; "block_ptr";
+   "bpf_state"; "state_pc"; "bpf_flag"; "mem_num"; "regsmap"; "mrs"] SymbolIRs.
