benchmark/clightlogicexample.v
@@ -1,0 +1,738 @@
+From Coq Require Import String List ZArith.
+From compcert Require Import Coqlib Integers Floats AST Ctypes Cop Clight Clightdefs.
+Import Clightdefs.ClightNotations.
+Local Open Scope Z_scope.
+Local Open Scope string_scope.
+Local Open Scope clight_scope.
+
+Module Info.
+  Definition version := "3.9".
+  Definition build_number := "".
+  Definition build_tag := "".
+  Definition build_branch := "".
+  Definition arch := "x86".
+  Definition model := "64".
+  Definition abi := "standard".
+  Definition bitsize := 64.
+  Definition big_endian := false.
+  Definition source_file := "clightlogicexample.c".
+  Definition normalized := false.
+End Info.
+
+Definition ___builtin_ais_annot : ident := $"__builtin_ais_annot".
+Definition ___builtin_annot : ident := $"__builtin_annot".
+Definition ___builtin_annot_intval : ident := $"__builtin_annot_intval".
+Definition ___builtin_bswap : ident := $"__builtin_bswap".
+Definition ___builtin_bswap16 : ident := $"__builtin_bswap16".
+Definition ___builtin_bswap32 : ident := $"__builtin_bswap32".
+Definition ___builtin_bswap64 : ident := $"__builtin_bswap64".
+Definition ___builtin_clz : ident := $"__builtin_clz".
+Definition ___builtin_clzl : ident := $"__builtin_clzl".
+Definition ___builtin_clzll : ident := $"__builtin_clzll".
+Definition ___builtin_ctz : ident := $"__builtin_ctz".
+Definition ___builtin_ctzl : ident := $"__builtin_ctzl".
+Definition ___builtin_ctzll : ident := $"__builtin_ctzll".
+Definition ___builtin_debug : ident := $"__builtin_debug".
+Definition ___builtin_expect : ident := $"__builtin_expect".
+Definition ___builtin_fabs : ident := $"__builtin_fabs".
+Definition ___builtin_fabsf : ident := $"__builtin_fabsf".
+Definition ___builtin_fmadd : ident := $"__builtin_fmadd".
+Definition ___builtin_fmax : ident := $"__builtin_fmax".
+Definition ___builtin_fmin : ident := $"__builtin_fmin".
+Definition ___builtin_fmsub : ident := $"__builtin_fmsub".
+Definition ___builtin_fnmadd : ident := $"__builtin_fnmadd".
+Definition ___builtin_fnmsub : ident := $"__builtin_fnmsub".
+Definition ___builtin_fsqrt : ident := $"__builtin_fsqrt".
+Definition ___builtin_membar : ident := $"__builtin_membar".
+Definition ___builtin_memcpy_aligned : ident := $"__builtin_memcpy_aligned".
+Definition ___builtin_read16_reversed : ident := $"__builtin_read16_reversed".
+Definition ___builtin_read32_reversed : ident := $"__builtin_read32_reversed".
+Definition ___builtin_sel : ident := $"__builtin_sel".
+Definition ___builtin_sqrt : ident := $"__builtin_sqrt".
+Definition ___builtin_unreachable : ident := $"__builtin_unreachable".
+Definition ___builtin_va_arg : ident := $"__builtin_va_arg".
+Definition ___builtin_va_copy : ident := $"__builtin_va_copy".
+Definition ___builtin_va_end : ident := $"__builtin_va_end".
+Definition ___builtin_va_start : ident := $"__builtin_va_start".
+Definition ___builtin_write16_reversed : ident := $"__builtin_write16_reversed".
+Definition ___builtin_write32_reversed : ident := $"__builtin_write32_reversed".
+Definition ___compcert_i64_dtos : ident := $"__compcert_i64_dtos".
+Definition ___compcert_i64_dtou : ident := $"__compcert_i64_dtou".
+Definition ___compcert_i64_sar : ident := $"__compcert_i64_sar".
+Definition ___compcert_i64_sdiv : ident := $"__compcert_i64_sdiv".
+Definition ___compcert_i64_shl : ident := $"__compcert_i64_shl".
+Definition ___compcert_i64_shr : ident := $"__compcert_i64_shr".
+Definition ___compcert_i64_smod : ident := $"__compcert_i64_smod".
+Definition ___compcert_i64_smulh : ident := $"__compcert_i64_smulh".
+Definition ___compcert_i64_stod : ident := $"__compcert_i64_stod".
+Definition ___compcert_i64_stof : ident := $"__compcert_i64_stof".
+Definition ___compcert_i64_udiv : ident := $"__compcert_i64_udiv".
+Definition ___compcert_i64_umod : ident := $"__compcert_i64_umod".
+Definition ___compcert_i64_umulh : ident := $"__compcert_i64_umulh".
+Definition ___compcert_i64_utod : ident := $"__compcert_i64_utod".
+Definition ___compcert_i64_utof : ident := $"__compcert_i64_utof".
+Definition ___compcert_va_composite : ident := $"__compcert_va_composite".
+Definition ___compcert_va_float64 : ident := $"__compcert_va_float64".
+Definition ___compcert_va_int32 : ident := $"__compcert_va_int32".
+Definition ___compcert_va_int64 : ident := $"__compcert_va_int64".
+Definition _block_perm : ident := $"block_perm".
+Definition _block_ptr : ident := $"block_ptr".
+Definition _block_size : ident := $"block_size".
+Definition _bpf_flag : ident := $"bpf_flag".
+Definition _bpf_state : ident := $"bpf_state".
+Definition _calc_sum : ident := $"calc_sum".
+Definition _chunk : ident := $"chunk".
+Definition _dst : ident := $"dst".
+Definition _eval_mem_regions : ident := $"eval_mem_regions".
+Definition _f : ident := $"f".
+Definition _get_add : ident := $"get_add".
+Definition _get_addr_ofs : ident := $"get_addr_ofs".
+Definition _get_immediate : ident := $"get_immediate".
+Definition _get_mem_region : ident := $"get_mem_region".
+Definition _get_opcode_mem_ld_imm : ident := $"get_opcode_mem_ld_imm".
+Definition _i : ident := $"i".
+Definition _idx : ident := $"idx".
+Definition _imm : ident := $"imm".
+Definition _ins : ident := $"ins".
+Definition _is_well_chunk_bool : ident := $"is_well_chunk_bool".
+Definition _l : ident := $"l".
+Definition _len : ident := $"len".
+Definition _list_get : ident := $"list_get".
+Definition _main : ident := $"main".
+Definition _mem_num : ident := $"mem_num".
+Definition _memory_region : ident := $"memory_region".
+Definition _mrs : ident := $"mrs".
+Definition _n : ident := $"n".
+Definition _n1 : ident := $"n1".
+Definition _next_imm : ident := $"next_imm".
+Definition _next_ins : ident := $"next_ins".
+Definition _nv : ident := $"nv".
+Definition _ofs : ident := $"ofs".
+Definition _op : ident := $"op".
+Definition _opcode_ld : ident := $"opcode_ld".
+Definition _pc : ident := $"pc".
+Definition _regsmap : ident := $"regsmap".
+Definition _st : ident := $"st".
+Definition _start_addr : ident := $"start_addr".
+Definition _state_pc : ident := $"state_pc".
+Definition _step_opcode_mem_ld_imm : ident := $"step_opcode_mem_ld_imm".
+Definition _upd_flag : ident := $"upd_flag".
+Definition _upd_pc_incr : ident := $"upd_pc_incr".
+Definition _upd_reg : ident := $"upd_reg".
+Definition _v : ident := $"v".
+Definition _x : ident := $"x".
+Definition _y : ident := $"y".
+Definition _t'1 : ident := 128%positive.
+Definition _t'2 : ident := 129%positive.
+Definition _t'3 : ident := 130%positive.
+
+Definition f_upd_pc_incr := {|
+  fn_return := tvoid;
+  fn_callconv := cc_default;
+  fn_params := ((_st, (tptr (Tstruct _bpf_state noattr))) :: nil);
+  fn_vars := nil;
+  fn_temps := nil;
+  fn_body :=
+(Ssequence
+  (Sassign
+    (Efield
+      (Ederef (Etempvar _st (tptr (Tstruct _bpf_state noattr)))
+        (Tstruct _bpf_state noattr)) _state_pc tuint)
+    (Ebinop Oadd
+      (Efield
+        (Ederef (Etempvar _st (tptr (Tstruct _bpf_state noattr)))
+          (Tstruct _bpf_state noattr)) _state_pc tuint)
+      (Econst_int (Int.repr 1) tint) tuint))
+  (Sreturn None))
+|}.
+
+Definition f_upd_reg := {|
+  fn_return := tvoid;
+  fn_callconv := cc_default;
+  fn_params := ((_st, (tptr (Tstruct _bpf_state noattr))) :: (_i, tuint) ::
+                (_v, tulong) :: nil);
+  fn_vars := nil;
+  fn_temps := nil;
+  fn_body :=
+(Ssequence
+  (Sassign
+    (Ederef
+      (Ebinop Oadd
+        (Efield
+          (Ederef (Etempvar _st (tptr (Tstruct _bpf_state noattr)))
+            (Tstruct _bpf_state noattr)) _regsmap (tarray tulong 11))
+        (Etempvar _i tuint) (tptr tulong)) tulong) (Etempvar _v tulong))
+  (Sreturn None))
+|}.
+
+Definition f_upd_flag := {|
+  fn_return := tvoid;
+  fn_callconv := cc_default;
+  fn_params := ((_st, (tptr (Tstruct _bpf_state noattr))) :: (_f, tint) ::
+                nil);
+  fn_vars := nil;
+  fn_temps := nil;
+  fn_body :=
+(Ssequence
+  (Sassign
+    (Efield
+      (Ederef (Etempvar _st (tptr (Tstruct _bpf_state noattr)))
+        (Tstruct _bpf_state noattr)) _bpf_flag tint) (Etempvar _f tint))
+  (Sreturn None))
+|}.
+
+Definition f_eval_mem_regions := {|
+  fn_return := (tptr (Tstruct _memory_region noattr));
+  fn_callconv := cc_default;
+  fn_params := ((_st, (tptr (Tstruct _bpf_state noattr))) :: nil);
+  fn_vars := nil;
+  fn_temps := nil;
+  fn_body :=
+(Sreturn (Some (Efield
+                 (Ederef (Etempvar _st (tptr (Tstruct _bpf_state noattr)))
+                   (Tstruct _bpf_state noattr)) _mrs
+                 (tptr (Tstruct _memory_region noattr)))))
+|}.
+
+Definition f_list_get := {|
+  fn_return := tulong;
+  fn_callconv := cc_default;
+  fn_params := ((_l, (tptr tulong)) :: (_idx, tint) :: nil);
+  fn_vars := nil;
+  fn_temps := nil;
+  fn_body :=
+(Sreturn (Some (Ederef
+                 (Ebinop Oadd (Etempvar _l (tptr tulong))
+                   (Etempvar _idx tint) (tptr tulong)) tulong)))
+|}.
+
+Definition f_get_mem_region := {|
+  fn_return := (tptr (Tstruct _memory_region noattr));
+  fn_callconv := cc_default;
+  fn_params := ((_st, (tptr (Tstruct _bpf_state noattr))) :: (_n, tuint) ::
+                nil);
+  fn_vars := nil;
+  fn_temps := ((_mrs, (tptr (Tstruct _memory_region noattr))) ::
+               (_t'1, (tptr (Tstruct _memory_region noattr))) :: nil);
+  fn_body :=
+(Ssequence
+  (Ssequence
+    (Scall (Some _t'1)
+      (Evar _eval_mem_regions (Tfunction
+                                (Tcons (tptr (Tstruct _bpf_state noattr))
+                                  Tnil)
+                                (tptr (Tstruct _memory_region noattr))
+                                cc_default))
+      ((Etempvar _st (tptr (Tstruct _bpf_state noattr))) :: nil))
+    (Sset _mrs (Etempvar _t'1 (tptr (Tstruct _memory_region noattr)))))
+  (Sreturn (Some (Ebinop Oadd
+                   (Etempvar _mrs (tptr (Tstruct _memory_region noattr)))
+                   (Etempvar _n tuint)
+                   (tptr (Tstruct _memory_region noattr))))))
+|}.
+
+Definition f_get_immediate := {|
+  fn_return := tint;
+  fn_callconv := cc_default;
+  fn_params := ((_ins, tulong) :: nil);
+  fn_vars := nil;
+  fn_temps := nil;
+  fn_body :=
+(Sreturn (Some (Ecast
+                 (Ebinop Oshr (Etempvar _ins tulong)
+                   (Econst_long (Int64.repr 32) tulong) tulong) tint)))
+|}.
+
+Definition f_get_opcode_mem_ld_imm := {|
+  fn_return := tuchar;
+  fn_callconv := cc_default;
+  fn_params := ((_op, tuchar) :: nil);
+  fn_vars := nil;
+  fn_temps := nil;
+  fn_body :=
+(Sreturn (Some (Ecast
+                 (Ebinop Oand (Etempvar _op tuchar)
+                   (Econst_int (Int.repr 255) tint) tint) tuchar)))
+|}.
+
+Definition f_get_add := {|
+  fn_return := tuint;
+  fn_callconv := cc_default;
+  fn_params := ((_x, tuint) :: (_y, tuint) :: nil);
+  fn_vars := nil;
+  fn_temps := nil;
+  fn_body :=
+(Sreturn (Some (Ebinop Oadd (Etempvar _x tuint) (Etempvar _y tuint) tuint)))
+|}.
+
+Definition f_get_addr_ofs := {|
+  fn_return := tuint;
+  fn_callconv := cc_default;
+  fn_params := ((_x, tulong) :: (_ofs, tint) :: nil);
+  fn_vars := nil;
+  fn_temps := nil;
+  fn_body :=
+(Sreturn (Some (Ecast
+                 (Ebinop Oadd (Etempvar _x tulong)
+                   (Ecast (Etempvar _ofs tint) tulong) tulong) tuint)))
+|}.
+
+Definition f_is_well_chunk_bool := {|
+  fn_return := tbool;
+  fn_callconv := cc_default;
+  fn_params := ((_chunk, tuint) :: nil);
+  fn_vars := nil;
+  fn_temps := nil;
+  fn_body :=
+(Sswitch (Etempvar _chunk tuint)
+  (LScons (Some 1)
+    (Sreturn (Some (Econst_int (Int.repr 1) tint)))
+    (LScons (Some 2)
+      (Sreturn (Some (Econst_int (Int.repr 1) tint)))
+      (LScons (Some 4)
+        (Sreturn (Some (Econst_int (Int.repr 1) tint)))
+        (LScons (Some 8)
+          (Sreturn (Some (Econst_int (Int.repr 1) tint)))
+          (LScons None (Sreturn (Some (Econst_int (Int.repr 0) tint))) LSnil))))))
+|}.
+
+Definition f_calc_sum := {|
+  fn_return := tuint;
+  fn_callconv := cc_default;
+  fn_params := ((_v, tuint) :: (_n, tuint) :: nil);
+  fn_vars := nil;
+  fn_temps := ((_n1, tuint) :: (_nv, tuint) :: (_t'2, tuint) ::
+               (_t'1, tuint) :: nil);
+  fn_body :=
+(Sifthenelse (Ebinop Oeq (Etempvar _n tuint) (Econst_int (Int.repr 0) tuint)
+               tint)
+  (Sreturn (Some (Econst_int (Int.repr 0) tuint)))
+  (Ssequence
+    (Sset _n1
+      (Ebinop Osub (Etempvar _n tuint) (Econst_int (Int.repr 1) tuint) tuint))
+    (Ssequence
+      (Ssequence
+        (Scall (Some _t'1)
+          (Evar _get_add (Tfunction (Tcons tuint (Tcons tuint Tnil)) tuint
+                           cc_default))
+          ((Etempvar _v tuint) :: (Econst_int (Int.repr 1) tuint) :: nil))
+        (Sset _nv (Etempvar _t'1 tuint)))
+      (Ssequence
+        (Scall (Some _t'2)
+          (Evar _calc_sum (Tfunction (Tcons tuint (Tcons tuint Tnil)) tuint
+                            cc_default))
+          ((Etempvar _nv tuint) :: (Etempvar _n1 tuint) :: nil))
+        (Sreturn (Some (Etempvar _t'2 tuint)))))))
+|}.
+
+Definition f_step_opcode_mem_ld_imm := {|
+  fn_return := tvoid;
+  fn_callconv := cc_default;
+  fn_params := ((_st, (tptr (Tstruct _bpf_state noattr))) :: (_imm, tint) ::
+                (_pc, tint) :: (_len, tint) :: (_dst, tuint) ::
+                (_op, tuchar) :: (_l, (tptr tulong)) :: nil);
+  fn_vars := nil;
+  fn_temps := ((_opcode_ld, tuchar) :: (_next_ins, tulong) ::
+               (_next_imm, tint) :: (_t'3, tint) :: (_t'2, tulong) ::
+               (_t'1, tuchar) :: nil);
+  fn_body :=
+(Ssequence
+  (Ssequence
+    (Scall (Some _t'1)
+      (Evar _get_opcode_mem_ld_imm (Tfunction (Tcons tuchar Tnil) tuchar
+                                     cc_default))
+      ((Etempvar _op tuchar) :: nil))
+    (Sset _opcode_ld (Ecast (Etempvar _t'1 tuchar) tuchar)))
+  (Sswitch (Etempvar _opcode_ld tuchar)
+    (LScons (Some 24)
+      (Sifthenelse (Ebinop Olt
+                     (Ebinop Oadd (Etempvar _pc tint)
+                       (Econst_int (Int.repr 1) tint) tint)
+                     (Etempvar _len tint) tint)
+        (Ssequence
+          (Ssequence
+            (Scall (Some _t'2)
+              (Evar _list_get (Tfunction
+                                (Tcons (tptr tulong) (Tcons tint Tnil))
+                                tulong cc_default))
+              ((Etempvar _l (tptr tulong)) ::
+               (Ebinop Oadd (Etempvar _pc tint)
+                 (Econst_int (Int.repr 1) tint) tint) :: nil))
+            (Sset _next_ins (Etempvar _t'2 tulong)))
+          (Ssequence
+            (Ssequence
+              (Scall (Some _t'3)
+                (Evar _get_immediate (Tfunction (Tcons tulong Tnil) tint
+                                       cc_default))
+                ((Etempvar _next_ins tulong) :: nil))
+              (Sset _next_imm (Etempvar _t'3 tint)))
+            (Ssequence
+              (Scall None
+                (Evar _upd_reg (Tfunction
+                                 (Tcons (tptr (Tstruct _bpf_state noattr))
+                                   (Tcons tuint (Tcons tulong Tnil))) tvoid
+                                 cc_default))
+                ((Etempvar _st (tptr (Tstruct _bpf_state noattr))) ::
+                 (Etempvar _dst tuint) ::
+                 (Ebinop Oor
+                   (Ecast (Ecast (Etempvar _imm tint) tuint) tulong)
+                   (Ebinop Oshl
+                     (Ecast (Ecast (Etempvar _next_imm tint) tuint) tulong)
+                     (Econst_int (Int.repr 32) tuint) tulong) tulong) :: nil))
+              (Ssequence
+                (Scall None
+                  (Evar _upd_pc_incr (Tfunction
+                                       (Tcons
+                                         (tptr (Tstruct _bpf_state noattr))
+                                         Tnil) tvoid cc_default))
+                  ((Etempvar _st (tptr (Tstruct _bpf_state noattr))) :: nil))
+                (Ssequence
+                  (Scall None
+                    (Evar _upd_flag (Tfunction
+                                      (Tcons
+                                        (tptr (Tstruct _bpf_state noattr))
+                                        (Tcons tint Tnil)) tvoid cc_default))
+                    ((Etempvar _st (tptr (Tstruct _bpf_state noattr))) ::
+                     (Econst_int (Int.repr 0) tint) :: nil))
+                  (Sreturn None))))))
+        (Ssequence
+          (Scall None
+            (Evar _upd_flag (Tfunction
+                              (Tcons (tptr (Tstruct _bpf_state noattr))
+                                (Tcons tint Tnil)) tvoid cc_default))
+            ((Etempvar _st (tptr (Tstruct _bpf_state noattr))) ::
+             (Eunop Oneg (Econst_int (Int.repr 5) tint) tint) :: nil))
+          (Sreturn None)))
+      (LScons None
+        (Ssequence
+          (Scall None
+            (Evar _upd_flag (Tfunction
+                              (Tcons (tptr (Tstruct _bpf_state noattr))
+                                (Tcons tint Tnil)) tvoid cc_default))
+            ((Etempvar _st (tptr (Tstruct _bpf_state noattr))) ::
+             (Eunop Oneg (Econst_int (Int.repr 1) tint) tint) :: nil))
+          (Sreturn None))
+        LSnil))))
+|}.
+
+Definition composites : list composite_definition :=
+(Composite _memory_region Struct
+   ((_start_addr, tuint) :: (_block_size, tuint) :: (_block_perm, tuint) ::
+    (_block_ptr, tuint) :: nil)
+   noattr ::
+ Composite _bpf_state Struct
+   ((_state_pc, tuint) :: (_bpf_flag, tint) :: (_mem_num, tuint) ::
+    (_regsmap, (tarray tulong 11)) ::
+    (_mrs, (tptr (Tstruct _memory_region noattr))) :: nil)
+   noattr :: nil).
+
+Definition global_definitions : list (ident * globdef fundef type) :=
+((___builtin_ais_annot,
+   Gfun(External (EF_builtin "__builtin_ais_annot"
+                   (mksignature (AST.Tlong :: nil) AST.Tvoid
+                     {|cc_vararg:=(Some 1); cc_unproto:=false; cc_structret:=false|}))
+     (Tcons (tptr tschar) Tnil) tvoid
+     {|cc_vararg:=(Some 1); cc_unproto:=false; cc_structret:=false|})) ::
+ (___builtin_bswap64,
+   Gfun(External (EF_builtin "__builtin_bswap64"
+                   (mksignature (AST.Tlong :: nil) AST.Tlong cc_default))
+     (Tcons tulong Tnil) tulong cc_default)) ::
+ (___builtin_bswap,
+   Gfun(External (EF_builtin "__builtin_bswap"
+                   (mksignature (AST.Tint :: nil) AST.Tint cc_default))
+     (Tcons tuint Tnil) tuint cc_default)) ::
+ (___builtin_bswap32,
+   Gfun(External (EF_builtin "__builtin_bswap32"
+                   (mksignature (AST.Tint :: nil) AST.Tint cc_default))
+     (Tcons tuint Tnil) tuint cc_default)) ::
+ (___builtin_bswap16,
+   Gfun(External (EF_builtin "__builtin_bswap16"
+                   (mksignature (AST.Tint :: nil) AST.Tint16unsigned
+                     cc_default)) (Tcons tushort Tnil) tushort cc_default)) ::
+ (___builtin_clz,
+   Gfun(External (EF_builtin "__builtin_clz"
+                   (mksignature (AST.Tint :: nil) AST.Tint cc_default))
+     (Tcons tuint Tnil) tint cc_default)) ::
+ (___builtin_clzl,
+   Gfun(External (EF_builtin "__builtin_clzl"
+                   (mksignature (AST.Tlong :: nil) AST.Tint cc_default))
+     (Tcons tulong Tnil) tint cc_default)) ::
+ (___builtin_clzll,
+   Gfun(External (EF_builtin "__builtin_clzll"
+                   (mksignature (AST.Tlong :: nil) AST.Tint cc_default))
+     (Tcons tulong Tnil) tint cc_default)) ::
+ (___builtin_ctz,
+   Gfun(External (EF_builtin "__builtin_ctz"
+                   (mksignature (AST.Tint :: nil) AST.Tint cc_default))
+     (Tcons tuint Tnil) tint cc_default)) ::
+ (___builtin_ctzl,
+   Gfun(External (EF_builtin "__builtin_ctzl"
+                   (mksignature (AST.Tlong :: nil) AST.Tint cc_default))
+     (Tcons tulong Tnil) tint cc_default)) ::
+ (___builtin_ctzll,
+   Gfun(External (EF_builtin "__builtin_ctzll"
+                   (mksignature (AST.Tlong :: nil) AST.Tint cc_default))
+     (Tcons tulong Tnil) tint cc_default)) ::
+ (___builtin_fabs,
+   Gfun(External (EF_builtin "__builtin_fabs"
+                   (mksignature (AST.Tfloat :: nil) AST.Tfloat cc_default))
+     (Tcons tdouble Tnil) tdouble cc_default)) ::
+ (___builtin_fabsf,
+   Gfun(External (EF_builtin "__builtin_fabsf"
+                   (mksignature (AST.Tsingle :: nil) AST.Tsingle cc_default))
+     (Tcons tfloat Tnil) tfloat cc_default)) ::
+ (___builtin_fsqrt,
+   Gfun(External (EF_builtin "__builtin_fsqrt"
+                   (mksignature (AST.Tfloat :: nil) AST.Tfloat cc_default))
+     (Tcons tdouble Tnil) tdouble cc_default)) ::
+ (___builtin_sqrt,
+   Gfun(External (EF_builtin "__builtin_sqrt"
+                   (mksignature (AST.Tfloat :: nil) AST.Tfloat cc_default))
+     (Tcons tdouble Tnil) tdouble cc_default)) ::
+ (___builtin_memcpy_aligned,
+   Gfun(External (EF_builtin "__builtin_memcpy_aligned"
+                   (mksignature
+                     (AST.Tlong :: AST.Tlong :: AST.Tlong :: AST.Tlong ::
+                      nil) AST.Tvoid cc_default))
+     (Tcons (tptr tvoid)
+       (Tcons (tptr tvoid) (Tcons tulong (Tcons tulong Tnil)))) tvoid
+     cc_default)) ::
+ (___builtin_sel,
+   Gfun(External (EF_builtin "__builtin_sel"
+                   (mksignature (AST.Tint :: nil) AST.Tvoid
+                     {|cc_vararg:=(Some 1); cc_unproto:=false; cc_structret:=false|}))
+     (Tcons tbool Tnil) tvoid
+     {|cc_vararg:=(Some 1); cc_unproto:=false; cc_structret:=false|})) ::
+ (___builtin_annot,
+   Gfun(External (EF_builtin "__builtin_annot"
+                   (mksignature (AST.Tlong :: nil) AST.Tvoid
+                     {|cc_vararg:=(Some 1); cc_unproto:=false; cc_structret:=false|}))
+     (Tcons (tptr tschar) Tnil) tvoid
+     {|cc_vararg:=(Some 1); cc_unproto:=false; cc_structret:=false|})) ::
+ (___builtin_annot_intval,
+   Gfun(External (EF_builtin "__builtin_annot_intval"
+                   (mksignature (AST.Tlong :: AST.Tint :: nil) AST.Tint
+                     cc_default)) (Tcons (tptr tschar) (Tcons tint Tnil))
+     tint cc_default)) ::
+ (___builtin_membar,
+   Gfun(External (EF_builtin "__builtin_membar"
+                   (mksignature nil AST.Tvoid cc_default)) Tnil tvoid
+     cc_default)) ::
+ (___builtin_va_start,
+   Gfun(External (EF_builtin "__builtin_va_start"
+                   (mksignature (AST.Tlong :: nil) AST.Tvoid cc_default))
+     (Tcons (tptr tvoid) Tnil) tvoid cc_default)) ::
+ (___builtin_va_arg,
+   Gfun(External (EF_builtin "__builtin_va_arg"
+                   (mksignature (AST.Tlong :: AST.Tint :: nil) AST.Tvoid
+                     cc_default)) (Tcons (tptr tvoid) (Tcons tuint Tnil))
+     tvoid cc_default)) ::
+ (___builtin_va_copy,
+   Gfun(External (EF_builtin "__builtin_va_copy"
+                   (mksignature (AST.Tlong :: AST.Tlong :: nil) AST.Tvoid
+                     cc_default))
+     (Tcons (tptr tvoid) (Tcons (tptr tvoid) Tnil)) tvoid cc_default)) ::
+ (___builtin_va_end,
+   Gfun(External (EF_builtin "__builtin_va_end"
+                   (mksignature (AST.Tlong :: nil) AST.Tvoid cc_default))
+     (Tcons (tptr tvoid) Tnil) tvoid cc_default)) ::
+ (___compcert_va_int32,
+   Gfun(External (EF_external "__compcert_va_int32"
+                   (mksignature (AST.Tlong :: nil) AST.Tint cc_default))
+     (Tcons (tptr tvoid) Tnil) tuint cc_default)) ::
+ (___compcert_va_int64,
+   Gfun(External (EF_external "__compcert_va_int64"
+                   (mksignature (AST.Tlong :: nil) AST.Tlong cc_default))
+     (Tcons (tptr tvoid) Tnil) tulong cc_default)) ::
+ (___compcert_va_float64,
+   Gfun(External (EF_external "__compcert_va_float64"
+                   (mksignature (AST.Tlong :: nil) AST.Tfloat cc_default))
+     (Tcons (tptr tvoid) Tnil) tdouble cc_default)) ::
+ (___compcert_va_composite,
+   Gfun(External (EF_external "__compcert_va_composite"
+                   (mksignature (AST.Tlong :: AST.Tlong :: nil) AST.Tlong
+                     cc_default)) (Tcons (tptr tvoid) (Tcons tulong Tnil))
+     (tptr tvoid) cc_default)) ::
+ (___builtin_unreachable,
+   Gfun(External (EF_builtin "__builtin_unreachable"
+                   (mksignature nil AST.Tvoid cc_default)) Tnil tvoid
+     cc_default)) ::
+ (___builtin_expect,
+   Gfun(External (EF_builtin "__builtin_expect"
+                   (mksignature (AST.Tlong :: AST.Tlong :: nil) AST.Tlong
+                     cc_default)) (Tcons tlong (Tcons tlong Tnil)) tlong
+     cc_default)) ::
+ (___compcert_i64_dtos,
+   Gfun(External (EF_runtime "__compcert_i64_dtos"
+                   (mksignature (AST.Tfloat :: nil) AST.Tlong cc_default))
+     (Tcons tdouble Tnil) tlong cc_default)) ::
+ (___compcert_i64_dtou,
+   Gfun(External (EF_runtime "__compcert_i64_dtou"
+                   (mksignature (AST.Tfloat :: nil) AST.Tlong cc_default))
+     (Tcons tdouble Tnil) tulong cc_default)) ::
+ (___compcert_i64_stod,
+   Gfun(External (EF_runtime "__compcert_i64_stod"
+                   (mksignature (AST.Tlong :: nil) AST.Tfloat cc_default))
+     (Tcons tlong Tnil) tdouble cc_default)) ::
+ (___compcert_i64_utod,
+   Gfun(External (EF_runtime "__compcert_i64_utod"
+                   (mksignature (AST.Tlong :: nil) AST.Tfloat cc_default))
+     (Tcons tulong Tnil) tdouble cc_default)) ::
+ (___compcert_i64_stof,
+   Gfun(External (EF_runtime "__compcert_i64_stof"
+                   (mksignature (AST.Tlong :: nil) AST.Tsingle cc_default))
+     (Tcons tlong Tnil) tfloat cc_default)) ::
+ (___compcert_i64_utof,
+   Gfun(External (EF_runtime "__compcert_i64_utof"
+                   (mksignature (AST.Tlong :: nil) AST.Tsingle cc_default))
+     (Tcons tulong Tnil) tfloat cc_default)) ::
+ (___compcert_i64_sdiv,
+   Gfun(External (EF_runtime "__compcert_i64_sdiv"
+                   (mksignature (AST.Tlong :: AST.Tlong :: nil) AST.Tlong
+                     cc_default)) (Tcons tlong (Tcons tlong Tnil)) tlong
+     cc_default)) ::
+ (___compcert_i64_udiv,
+   Gfun(External (EF_runtime "__compcert_i64_udiv"
+                   (mksignature (AST.Tlong :: AST.Tlong :: nil) AST.Tlong
+                     cc_default)) (Tcons tulong (Tcons tulong Tnil)) tulong
+     cc_default)) ::
+ (___compcert_i64_smod,
+   Gfun(External (EF_runtime "__compcert_i64_smod"
+                   (mksignature (AST.Tlong :: AST.Tlong :: nil) AST.Tlong
+                     cc_default)) (Tcons tlong (Tcons tlong Tnil)) tlong
+     cc_default)) ::
+ (___compcert_i64_umod,
+   Gfun(External (EF_runtime "__compcert_i64_umod"
+                   (mksignature (AST.Tlong :: AST.Tlong :: nil) AST.Tlong
+                     cc_default)) (Tcons tulong (Tcons tulong Tnil)) tulong
+     cc_default)) ::
+ (___compcert_i64_shl,
+   Gfun(External (EF_runtime "__compcert_i64_shl"
+                   (mksignature (AST.Tlong :: AST.Tint :: nil) AST.Tlong
+                     cc_default)) (Tcons tlong (Tcons tint Tnil)) tlong
+     cc_default)) ::
+ (___compcert_i64_shr,
+   Gfun(External (EF_runtime "__compcert_i64_shr"
+                   (mksignature (AST.Tlong :: AST.Tint :: nil) AST.Tlong
+                     cc_default)) (Tcons tulong (Tcons tint Tnil)) tulong
+     cc_default)) ::
+ (___compcert_i64_sar,
+   Gfun(External (EF_runtime "__compcert_i64_sar"
+                   (mksignature (AST.Tlong :: AST.Tint :: nil) AST.Tlong
+                     cc_default)) (Tcons tlong (Tcons tint Tnil)) tlong
+     cc_default)) ::
+ (___compcert_i64_smulh,
+   Gfun(External (EF_runtime "__compcert_i64_smulh"
+                   (mksignature (AST.Tlong :: AST.Tlong :: nil) AST.Tlong
+                     cc_default)) (Tcons tlong (Tcons tlong Tnil)) tlong
+     cc_default)) ::
+ (___compcert_i64_umulh,
+   Gfun(External (EF_runtime "__compcert_i64_umulh"
+                   (mksignature (AST.Tlong :: AST.Tlong :: nil) AST.Tlong
+                     cc_default)) (Tcons tulong (Tcons tulong Tnil)) tulong
+     cc_default)) ::
+ (___builtin_fmax,
+   Gfun(External (EF_builtin "__builtin_fmax"
+                   (mksignature (AST.Tfloat :: AST.Tfloat :: nil) AST.Tfloat
+                     cc_default)) (Tcons tdouble (Tcons tdouble Tnil))
+     tdouble cc_default)) ::
+ (___builtin_fmin,
+   Gfun(External (EF_builtin "__builtin_fmin"
+                   (mksignature (AST.Tfloat :: AST.Tfloat :: nil) AST.Tfloat
+                     cc_default)) (Tcons tdouble (Tcons tdouble Tnil))
+     tdouble cc_default)) ::
+ (___builtin_fmadd,
+   Gfun(External (EF_builtin "__builtin_fmadd"
+                   (mksignature
+                     (AST.Tfloat :: AST.Tfloat :: AST.Tfloat :: nil)
+                     AST.Tfloat cc_default))
+     (Tcons tdouble (Tcons tdouble (Tcons tdouble Tnil))) tdouble
+     cc_default)) ::
+ (___builtin_fmsub,
+   Gfun(External (EF_builtin "__builtin_fmsub"
+                   (mksignature
+                     (AST.Tfloat :: AST.Tfloat :: AST.Tfloat :: nil)
+                     AST.Tfloat cc_default))
+     (Tcons tdouble (Tcons tdouble (Tcons tdouble Tnil))) tdouble
+     cc_default)) ::
+ (___builtin_fnmadd,
+   Gfun(External (EF_builtin "__builtin_fnmadd"
+                   (mksignature
+                     (AST.Tfloat :: AST.Tfloat :: AST.Tfloat :: nil)
+                     AST.Tfloat cc_default))
+     (Tcons tdouble (Tcons tdouble (Tcons tdouble Tnil))) tdouble
+     cc_default)) ::
+ (___builtin_fnmsub,
+   Gfun(External (EF_builtin "__builtin_fnmsub"
+                   (mksignature
+                     (AST.Tfloat :: AST.Tfloat :: AST.Tfloat :: nil)
+                     AST.Tfloat cc_default))
+     (Tcons tdouble (Tcons tdouble (Tcons tdouble Tnil))) tdouble
+     cc_default)) ::
+ (___builtin_read16_reversed,
+   Gfun(External (EF_builtin "__builtin_read16_reversed"
+                   (mksignature (AST.Tlong :: nil) AST.Tint16unsigned
+                     cc_default)) (Tcons (tptr tushort) Tnil) tushort
+     cc_default)) ::
+ (___builtin_read32_reversed,
+   Gfun(External (EF_builtin "__builtin_read32_reversed"
+                   (mksignature (AST.Tlong :: nil) AST.Tint cc_default))
+     (Tcons (tptr tuint) Tnil) tuint cc_default)) ::
+ (___builtin_write16_reversed,
+   Gfun(External (EF_builtin "__builtin_write16_reversed"
+                   (mksignature (AST.Tlong :: AST.Tint :: nil) AST.Tvoid
+                     cc_default)) (Tcons (tptr tushort) (Tcons tushort Tnil))
+     tvoid cc_default)) ::
+ (___builtin_write32_reversed,
+   Gfun(External (EF_builtin "__builtin_write32_reversed"
+                   (mksignature (AST.Tlong :: AST.Tint :: nil) AST.Tvoid
+                     cc_default)) (Tcons (tptr tuint) (Tcons tuint Tnil))
+     tvoid cc_default)) ::
+ (___builtin_debug,
+   Gfun(External (EF_external "__builtin_debug"
+                   (mksignature (AST.Tint :: nil) AST.Tvoid
+                     {|cc_vararg:=(Some 1); cc_unproto:=false; cc_structret:=false|}))
+     (Tcons tint Tnil) tvoid
+     {|cc_vararg:=(Some 1); cc_unproto:=false; cc_structret:=false|})) ::
+ (_upd_pc_incr, Gfun(Internal f_upd_pc_incr)) ::
+ (_upd_reg, Gfun(Internal f_upd_reg)) ::
+ (_upd_flag, Gfun(Internal f_upd_flag)) ::
+ (_eval_mem_regions, Gfun(Internal f_eval_mem_regions)) ::
+ (_list_get, Gfun(Internal f_list_get)) ::
+ (_get_mem_region, Gfun(Internal f_get_mem_region)) ::
+ (_get_immediate, Gfun(Internal f_get_immediate)) ::
+ (_get_opcode_mem_ld_imm, Gfun(Internal f_get_opcode_mem_ld_imm)) ::
+ (_get_add, Gfun(Internal f_get_add)) ::
+ (_get_addr_ofs, Gfun(Internal f_get_addr_ofs)) ::
+ (_is_well_chunk_bool, Gfun(Internal f_is_well_chunk_bool)) ::
+ (_calc_sum, Gfun(Internal f_calc_sum)) ::
+ (_step_opcode_mem_ld_imm, Gfun(Internal f_step_opcode_mem_ld_imm)) :: nil).
+
+Definition public_idents : list ident :=
+(_step_opcode_mem_ld_imm :: _calc_sum :: _is_well_chunk_bool ::
+ _get_addr_ofs :: _get_add :: _get_opcode_mem_ld_imm :: _get_immediate ::
+ _get_mem_region :: _list_get :: ___builtin_debug ::
+ ___builtin_write32_reversed :: ___builtin_write16_reversed ::
+ ___builtin_read32_reversed :: ___builtin_read16_reversed ::
+ ___builtin_fnmsub :: ___builtin_fnmadd :: ___builtin_fmsub ::
+ ___builtin_fmadd :: ___builtin_fmin :: ___builtin_fmax ::
+ ___compcert_i64_umulh :: ___compcert_i64_smulh :: ___compcert_i64_sar ::
+ ___compcert_i64_shr :: ___compcert_i64_shl :: ___compcert_i64_umod ::
+ ___compcert_i64_smod :: ___compcert_i64_udiv :: ___compcert_i64_sdiv ::
+ ___compcert_i64_utof :: ___compcert_i64_stof :: ___compcert_i64_utod ::
+ ___compcert_i64_stod :: ___compcert_i64_dtou :: ___compcert_i64_dtos ::
+ ___builtin_expect :: ___builtin_unreachable :: ___compcert_va_composite ::
+ ___compcert_va_float64 :: ___compcert_va_int64 :: ___compcert_va_int32 ::
+ ___builtin_va_end :: ___builtin_va_copy :: ___builtin_va_arg ::
+ ___builtin_va_start :: ___builtin_membar :: ___builtin_annot_intval ::
+ ___builtin_annot :: ___builtin_sel :: ___builtin_memcpy_aligned ::
+ ___builtin_sqrt :: ___builtin_fsqrt :: ___builtin_fabsf ::
+ ___builtin_fabs :: ___builtin_ctzll :: ___builtin_ctzl :: ___builtin_ctz ::
+ ___builtin_clzll :: ___builtin_clzl :: ___builtin_clz ::
+ ___builtin_bswap16 :: ___builtin_bswap32 :: ___builtin_bswap ::
+ ___builtin_bswap64 :: ___builtin_ais_annot :: nil).
+
+Definition prog : Clight.program := 
+  mkprogram composites global_definitions public_idents _main Logic.I.
+
+
