benchmark/correct_get_addr_ofs.v
@@ -1,0 +1,117 @@
+From bpf.src Require Import DxIntegers DxValues DxMemRegion DxState DxMonad DxInstructions.
+From Coq Require Import List Lia.
+From compcert Require Import Integers Values Clight Memory.
+Import ListNotations.
+Require Import ZArith.
+
+From bpf.proof Require Import Clightlogic MatchState CorrectRel CommonLemma.
+
+From bpf.benchmark Require Import clightlogicexample.
+
+
+(**
+unsigned int get_addr_ofs(unsigned long long x, int ofs)
+{
+  return (unsigned int) (x + (unsigned long long) ofs);
+}
+
+Print get_addr_ofs.
+get_addr_ofs = 
+fun (x : val64_t) (ofs : sint32_t) =>
+returnM (val_intuoflongu (Val.addl x (Val.longofintu (sint32_to_vint ofs))))
+     : val64_t -> sint32_t -> M valu32_t
+
+*)
+
+Section Get_addr_ofs.
+
+  (** The program contains our function of interest [fn] *)
+  Definition p : Clight.program := prog.
+
+  (* [Args,Res] provides the mapping between the Coq and the C types *)
+  (* Definition Args : list CompilableType := [stateCompilableType].*)
+  Definition args : list Type := [(val64_t:Type); (sint32_t:Type)].
+  Definition res : Type := (valu32_t:Type).
+
+  (* [f] is a Coq Monadic function with the right type *)
+  Definition f : arrow_type args (M res) := get_addr_ofs.
+
+  Variable state_block: block. (**r a block storing all rbpf state information? *)
+
+  (* [fn] is the Cligth function which has the same behaviour as [f] *)
+  Definition fn: Clight.function := f_get_addr_ofs.
+
+  (* [match_arg] relates the Coq arguments and the C arguments *)
+  Definition match_arg_list : DList.t (fun x => x -> val -> stateM -> Memory.Mem.mem -> Prop) args :=
+    (DList.DCons (stateless val64_correct)
+       (DList.DCons (stateless sint32_correct)
+                    (DList.DNil _))).
+
+  (* [match_res] relates the Coq result and the C result *)
+  Definition match_res : res -> val -> stateM -> Memory.Mem.mem -> Prop := fun x v st m => valu32_correct x v.
+
+  Instance correct_function3_get_addr_ofs : correct_function3 p args res f fn (nil) true match_arg_list match_res.
+  Proof.
+    correct_function_from_body.
+    correct_body.
+    (** how to use correct_* *)
+    unfold INV.
+    unfold f.
+    repeat intro.
+    get_invariant_more _x.
+    get_invariant_more _ofs.
+
+    unfold stateless, val64_correct in H1.
+    unfold stateless, sint32_correct in H3.
+    destruct H1 as (Hc_eq & (vi & Hvi_eq)).
+    subst c v v0.
+
+    (**according to the type of eval_pc:
+unsigned int get_addr_ofs(unsigned long long x, int ofs)
+{
+  return (unsigned int) (x + (unsigned long long) ofs);
+}
+       1. return value should be  x+y
+       2. the memory is same
+      *)
+    eexists. exists m, Events.E0.
+
+    repeat split; unfold step2.
+    -
+      apply Smallstep.plus_star.
+      (** TODO: adding Sreturn  more info by Ltac2 *)
+      eapply Smallstep.plus_one; eauto.
+      eapply step_return_1.
+      +
+        repeat econstructor; eauto.
+        simpl.
+        Transparent Archi.ptr64.
+        unfold Cop.sem_cast, Cop.classify_cast; simpl.
+        reflexivity.
+        unfold Cop.sem_binary_operation.
+        unfold Cop.sem_add, Cop.classify_add, Ctypes.typeconv; simpl.
+        unfold Cop.sem_binarith, Cop.sem_cast, Cop.classify_cast; simpl.
+        (**r we need a 32 Arch.
+match
+  match (if Archi.ptr64 then Cop.cast_case_pointer else Cop.cast_case_l2l) with
+  | Cop.cast_case_pointer => if Archi.ptr64 then None
+
+*)
+        reflexivity.
+        unfold Cop.sem_cast, Cop.classify_cast; simpl.
+        reflexivity.
+      +
+        unfold Cop.sem_cast, Cop.classify_cast; simpl.
+        reflexivity.
+      + 
+        econstructor; eauto.
+    - simpl.
+      eexists; reflexivity.
+    - simpl.
+      constructor.
+      reflexivity.
+  Qed.
+
+End Get_addr_ofs.
+
+Existing Instance correct_function3_get_addr_ofs.
