src/DxMonad.v
@@ -1,5 +1,5 @@
 From compcert Require Import AST Memory.
-Require Import DxIntegers DxValues DxRegs DxFlag DxMemRegion DxState.
+From bpf.src Require Import DxIntegers DxValues DxRegs DxFlag DxMemRegion DxState.
 
 
 Definition stateM := state. (*This one must be int_64 defined in DxIntegers *)
