Makefile
@@ -20,7 +20,7 @@ THIS_FILE := $(lastword $(MAKEFILE_LIST))
 COQPROJOPTS := $(shell $(CAT) _CoqProject)
 COQDEPOPTS := $(COQPROJOPTS)
 COQCOPTS := $(COQPROJOPTS) -w all,-notation
-COQEXTROPTS :=  -R ../tests dx.tests -w all,-extraction
+COQEXTROPTS :=  -R ../src dx.src -w all,-extraction
 
 OCAMLINCS := -I extr # -I src
 
@@ -40,14 +40,44 @@ test:
 	@$(MAKE) extract
 	@$(MAKE) repatch
 
-COQSRC = $(wildcard tests/*.v)
+BENCHSRC = $(wildcard benchmark/*.v)
+
+bench:
+	@echo $@
+	$(COQMAKEFILE) -f _CoqProject $(BENCHSRC) COQEXTRAFLAGS = '-w all,-extraction'  -o CoqMakefile
+	make -f CoqMakefile
+	$(CP) BenchmarkTestMain.ml benchmark
+	$(CP) BenchmarkTestMain.mli benchmark
+	$(COMPCERTSRCDIR)/tools/modorder $(COMPCERTSRCDIR)/.depend.extr cfrontend/PrintCsyntax.cmx | \
+	    $(AWK) '{ delete paths ;                                                                 \
+	              for(i = 1; i <= NF; i++) {                                                     \
+	                 x = $$i ;                                                                   \
+	                 sub("/[^/]*$$", "", x) ;                                                    \
+	                 paths[x] = 1 ;                                                              \
+	              }                                                                              \
+	              for(p in paths) {                                                              \
+	                 print "-I" ;                                                                \
+	                 print "$(COMPCERTSRCDIR)/" p ;                                              \
+	              }                                                                              \
+	            }' > compcertsrc-I	
+	$(COMPCERTSRCDIR)/tools/modorder $(COMPCERTSRCDIR)/.depend.extr cfrontend/PrintCsyntax.cmx | \
+	    $(AWK) 'BEGIN { RS=" " } /cmx/ { gsub(".*/","") ; print }' > compcertcprinter-cmx-args
+	$(OCAMLOPT) -args compcertsrc-I -I $(DXDIR)/extr -I $(DXDIR)/src -I benchmark benchmark/BenchmarkTestMain.mli	
+	$(OCAMLOPT) -args compcertsrc-I -I $(DXDIR)/extr -I $(DXDIR)/src -I benchmark -c benchmark/BenchmarkTestMain.ml
+	$(OCAMLOPT) -args compcertsrc-I -a -args compcertcprinter-cmx-args -o compcertcprinter.cmxa
+	$(OCAMLOPT) -args compcertsrc-I -a -args compcertcprinter-cmx-args -o compcertcprinter.a
+	$(OCAMLOPT) -args compcertsrc-I str.cmxa unix.cmxa compcertcprinter.cmxa $(DXDIR)/extr/ResultMonad.cmx $(DXDIR)/extr/DXModule.cmx $(DXDIR)/extr/DumpAsC.cmx benchmark/BenchmarkTestMain.cmx -o benchmark/main
+	ln -sf $(COMPCERTSRCDIR)/compcert.ini benchmark/compcert.ini
+	cd benchmark && ./main
+
+COQSRC = $(wildcard src/*.v)
 
 compile:
 	@echo $@
 	$(COQMAKEFILE) -f _CoqProject $(COQSRC) COQEXTRAFLAGS = '-w all,-extraction'  -o CoqMakefile
 	make -f CoqMakefile
-	$(CP) TestMain.ml tests # mv -> cp to avoid when running `make` again, it doesn't find the two files
-	$(CP) TestMain.mli tests
+	$(CP) TestMain.ml src # mv -> cp to avoid when running `make` again, it doesn't find the two files
+	$(CP) TestMain.mli src
 
 extract:
 	@echo $@
@@ -65,17 +95,17 @@ extract:
 	            }' > compcertsrc-I	
 	$(COMPCERTSRCDIR)/tools/modorder $(COMPCERTSRCDIR)/.depend.extr cfrontend/PrintCsyntax.cmx | \
 	    $(AWK) 'BEGIN { RS=" " } /cmx/ { gsub(".*/","") ; print }' > compcertcprinter-cmx-args
-	$(OCAMLOPT) -args compcertsrc-I -I $(DXDIR)/extr -I $(DXDIR)/src -I tests tests/TestMain.mli	
-	$(OCAMLOPT) -args compcertsrc-I -I $(DXDIR)/extr -I $(DXDIR)/src -I tests -c tests/TestMain.ml
+	$(OCAMLOPT) -args compcertsrc-I -I $(DXDIR)/extr -I $(DXDIR)/src -I src src/TestMain.mli	
+	$(OCAMLOPT) -args compcertsrc-I -I $(DXDIR)/extr -I $(DXDIR)/src -I src -c src/TestMain.ml
 	$(OCAMLOPT) -args compcertsrc-I -a -args compcertcprinter-cmx-args -o compcertcprinter.cmxa
 	$(OCAMLOPT) -args compcertsrc-I -a -args compcertcprinter-cmx-args -o compcertcprinter.a
-	$(OCAMLOPT) -args compcertsrc-I str.cmxa unix.cmxa compcertcprinter.cmxa $(DXDIR)/extr/ResultMonad.cmx $(DXDIR)/extr/DXModule.cmx $(DXDIR)/extr/DumpAsC.cmx tests/TestMain.cmx -o tests/main
-	ln -sf $(COMPCERTSRCDIR)/compcert.ini tests/compcert.ini
-	cd tests && ./main
+	$(OCAMLOPT) -args compcertsrc-I str.cmxa unix.cmxa compcertcprinter.cmxa $(DXDIR)/extr/ResultMonad.cmx $(DXDIR)/extr/DXModule.cmx $(DXDIR)/extr/DumpAsC.cmx src/TestMain.cmx -o src/main
+	ln -sf $(COMPCERTSRCDIR)/compcert.ini src/compcert.ini
+	cd src && ./main
 
 repatch:
 	@echo $@
-	$(CP) tests/generated.c repatch
+	$(CP) src/generated.c repatch
 	cd repatch && $(CC) -o repatch1 repatch1.c && ./repatch1 && $(CC) -o repatch2 repatch2.c && ./repatch2 && $(CC) -o repatch3 repatch3.c && ./repatch3 && $(CC) -o repatch4 repatch4.c && ./repatch4
 	$(CP) repatch/interpreter.c clight
 
@@ -85,7 +115,7 @@ clight:
 	cd clight && $(CLIGHTGEN) interpreter.c
 	$(CP) clight/interpreter.v codeTest
 
-PROOF = $(addprefix codeTest/,clight_exec.v Clightlogic.v interpreter.v CommonLemma.v MatchState.v CorrectRel.v correct_is_well_chunk_bool.v correct_upd_pc.v correct_eval_pc.v correct_upd_pc_incr.v correct_eval_reg.v correct_upd_reg.v correct_eval_flag.v correct_upd_flag.v correct_getMemRegion_block_ptr.v correct_getMemRegion_block_size.v correct_getMemRegion_start_addr.v correct_get_addl.v correct_get_subl.v correct_check_mem_aux.v)
+PROOF = $(addprefix proof/,clight_exec.v Clightlogic.v interpreter.v CommonLemma.v MatchState.v CorrectRel.v correct_is_well_chunk_bool.v correct_upd_pc.v correct_eval_pc.v correct_upd_pc_incr.v correct_eval_reg.v correct_upd_reg.v correct_eval_flag.v correct_upd_flag.v correct_getMemRegion_block_ptr.v correct_getMemRegion_block_size.v correct_getMemRegion_start_addr.v correct_get_addl.v correct_get_subl.v correct_check_mem_aux.v)
 
 proof:
 	@echo $@
@@ -102,4 +132,4 @@ clean :
 # We want to keep the .cmi that were built as we go
 .SECONDARY:
 
-.PHONY: all compile extract repatch clight proof clean
+.PHONY: all test bench compile extract repatch clight proof clean
